src/program_proof/wal/proof.v
@@ -60,14 +60,18 @@ Fixpoint compute_memLogMap (memLog : list update.t) (pos : u64) (m : gmap u64 va
 (** the lock invariant protecting the WalogState, corresponding to l.memLock *)
 Definition wal_linv (st: loc) γ : iProp Σ :=
   ∃ (memLogSlice : Slice.t)
+    (* TODO: group these into a Record *)
     (memLogMapPtr : loc)
     (memStart diskEnd nextDiskEnd : u64)
+    (shutdown:bool) (nthread: u64)
     (memLog : list update.t),
-    st ↦[WalogState.S :: "memLog"] (slice_val memLogSlice) ∗
-    st ↦[WalogState.S :: "memStart"] #memStart ∗
-    st ↦[WalogState.S :: "diskEnd"] #diskEnd ∗
-    st ↦[WalogState.S :: "nextDiskEnd"] #nextDiskEnd ∗
-    st ↦[WalogState.S :: "memLogMap"] #memLogMapPtr ∗
+    (st ↦[WalogState.S :: "memLog"] (slice_val memLogSlice) ∗
+     st ↦[WalogState.S :: "memStart"] #memStart ∗
+     st ↦[WalogState.S :: "diskEnd"] #diskEnd ∗
+     st ↦[WalogState.S :: "nextDiskEnd"] #nextDiskEnd ∗
+     st ↦[WalogState.S :: "memLogMap"] #memLogMapPtr ∗
+     st ↦[WalogState.S :: "shutdown"] #shutdown ∗
+     st ↦[WalogState.S :: "nthread"] #nthread) ∗
     (updates_slice memLogSlice memLog) ∗
     is_map memLogMapPtr (compute_memLogMap memLog memStart ∅, #0) ∗
     diskEnd_at_least γ.(circ_name) (int.val diskEnd) ∗
@@ -78,18 +82,16 @@ Definition wal_linv (st: loc) γ : iProp Σ :=
     .
 
 Definition is_wal_mem (l: loc) γ : iProp Σ :=
+  (* TODO: group these into a record *)
   ∃ (memLock : loc) (d : val) (circ st : loc)
-      (shutdown : bool) (nthread : u64)
       (condLogger condInstall condShut : loc),
-    (∃ q, (l ↦[Walog.S :: "memLock"]{q} #memLock ∗
+    (∃ q,  l ↦[Walog.S :: "memLock"]{q} #memLock ∗
            l ↦[Walog.S :: "d"]{q} d ∗
            l ↦[Walog.S :: "circ"]{q} #circ ∗
            l ↦[Walog.S :: "st"]{q} #st ∗
            l ↦[Walog.S :: "condLogger"]{q} #condLogger ∗
            l ↦[Walog.S :: "condInstall"]{q} #condInstall ∗
-           l ↦[Walog.S :: "condShut"]{q} #condShut ∗
-           l ↦[Walog.S :: "shutdown"]{q} #shutdown ∗
-           l ↦[Walog.S :: "nthread"]{q} #nthread)) ∗
+           l ↦[Walog.S :: "condShut"]{q} #condShut) ∗
     lock.is_cond condLogger #memLock ∗
     lock.is_cond condInstall #memLock ∗
     lock.is_cond condShut #memLock ∗
@@ -103,18 +105,18 @@ Proof.
   iIntros "Hinv".
   iDestruct "Hinv" as
       (memLock d circ st
-         shutdown nthread condLogger condInstall condShut)
+         condLogger condInstall condShut)
         "(Hfields&HcondLogger&HcondInstall&HcondShut&#His_lock)".
-  iDestruct "Hfields" as (q) "([Hf1 ?] & [Hf2 ?] & [Hf3 ?] & [Hf4 ?] & [Hf5 ?] & [Hf6 ?] & [Hf7 ?] & [Hf8 ?] & [Hf9 ?])".
+  iDestruct "Hfields" as (q) "([Hf1 ?] & [Hf2 ?] & [Hf3 ?] & [Hf4 ?] & [Hf5 ?] & [Hf6 ?] & [Hf7 ?])".
   iDestruct (is_cond_dup with "HcondLogger") as "[Hcond1 ?]".
   iDestruct (is_cond_dup with "HcondInstall") as "[Hcond2 ?]".
   iDestruct (is_cond_dup with "HcondShut") as "[Hcond3 ?]".
-  iSplitL "Hf1 Hf2 Hf3 Hf4 Hf5 Hf6 Hf7 Hf8 Hf9 Hcond1 Hcond2 Hcond3".
-  { iExists memLock, d, circ, st, shutdown, nthread.
+  iSplitL "Hf1 Hf2 Hf3 Hf4 Hf5 Hf6 Hf7 Hcond1 Hcond2 Hcond3".
+  { iExists memLock, d, circ, st.
     iExists condLogger, condInstall, condShut.
     iFrame "∗ His_lock".
     iExists (q/2)%Qp; iFrame. }
-  { iExists memLock, d, circ, st, shutdown, nthread.
+  { iExists memLock, d, circ, st.
     iExists condLogger, condInstall, condShut.
     iFrame "∗ His_lock".
     iExists (q/2)%Qp; iFrame. }
@@ -204,7 +206,7 @@ Definition is_memlog (s: log_state.t)
 Definition is_wal_inner (l : loc) γ s : iProp Σ :=
   ∃ (cs: circΣ.t) (memStart : u64)
        (memLog : list update.t)
-       (absorptionBoundaries : gmap nat unit) (γnextDiskEnd: gname),
+       (absorptionBoundaries : gmap nat unit),
     is_wal_mem l γ ∗
     own γ.(cs_name) (◯ (Excl' cs)) ∗
     own γ.(memStart_name) (◯ (Excl' memStart)) ∗
@@ -216,7 +218,7 @@ Definition is_wal_inner (l : loc) γ s : iProp Σ :=
        these conditions ensure that it is recorded as an absorption boundary,
        since at this point it becomes a plausible crash point *)
     ( ∃ (nextDiskEnd_txn_id : nat) (nextDiskEnd : u64),
-      own γnextDiskEnd (◯ (Excl' nextDiskEnd)) ∗
+      own γ.(nextDiskEnd_name) (◯ (Excl' nextDiskEnd)) ∗
       ⌜ absorptionBoundaries !! nextDiskEnd_txn_id = Some tt ⌝ ∗
       txn_pos s nextDiskEnd_txn_id nextDiskEnd ) ∗
     (* next, transactions are actually logged to the circ buffer *)
@@ -239,8 +241,52 @@ Definition is_wal_inner (l : loc) γ s : iProp Σ :=
       txn_pos s memStart_txn_id memStart ∗
       ⌜is_memlog s memStart_txn_id memLog absorptionBoundaries memStart⌝.
 
-Definition is_wal (l : loc) : iProp Σ :=
-  ∃ γ, inv walN (∃ σ, is_wal_inner l γ σ ∗ P σ) ∗
-    is_circular circN (circular_pred γ) γ.(circ_name).
+Definition is_wal (l : loc) γ : iProp Σ :=
+  inv walN (∃ σ, is_wal_inner l γ σ ∗ P σ) ∗
+  is_circular circN (circular_pred γ) γ.(circ_name).
+
+Instance is_cond_timeless (c l: loc) : Timeless (is_cond c #l).
+Proof.
+  rewrite /is_cond.
+  refine _.
+Qed.
+
+Theorem is_wal_read_mem l γ : is_wal l γ -∗ |={⊤}=> ▷ is_wal_mem l γ.
+Proof.
+  iIntros "#Hwal".
+  iDestruct "Hwal" as "[Hinv _]".
+  iApply (inv_dup_acc with "Hinv"); first by set_solver.
+  iIntros "HinvI".
+  iDestruct "HinvI" as (σ) "[HinvI HP]".
+  iDestruct "HinvI" as (cs memStart memLog absorptionBoundaries) "(Hmem&Hrest)".
+  iDestruct (is_wal_mem_dup with "Hmem") as "[Hmem1 Hmem2]".
+  iSplitR "Hmem2"; last by auto.
+  iExists _; iFrame.
+  iExists _, _, _, _; iFrame.
+Qed.
+
+Theorem wp_Walog__logger l γ :
+  {{{ is_wal l γ }}}
+    Walog__logger #l
+  {{{ RET #(); True }}}.
+Proof.
+  iIntros (Φ) "#Hwal HΦ".
+  iMod (is_wal_read_mem with "Hwal") as "Hmem".
+  wp_call.
+  iDestruct "Hmem" as (memLock d circ st condLogger condInstall condShut) "Hmem".
+  iDestruct "Hmem" as "(Hfields&HcondLogger&HcondInstall&HcondShut&Hlk)".
+  iDestruct "Hfields" as (q) "(Hf1&Hf2&Hf3&Hf4&Hf5&Hf6&Hf7)".
+  wp_loadField.
+  wp_apply (acquire_spec with "[$]").
+  iIntros "(Hlk_held&Hlkinv)".
+  iDestruct "Hlkinv" as (memLogSlice memLogMapPtr memStart diskEnd nextDiskEnd shutdown nthread memLog) "[Hfields Hrest]".
+  iDestruct "Hfields" as "(HmemLog&HmemStart&HdiskEnd&HnextDiskEnd&HmemLogMap&Hshutdown&Hnthread)".
+  wp_loadField.
+  wp_loadField.
+  wp_loadField.
+  wp_storeField.
+  wp_pures.
+  wp_bind (For _ _ _).
+Abort.
 
 End heap.
